ExistentialRules/ChaseSequence/CoreChase/Util.lean
@@ -4,6 +4,214 @@ import PossiblyInfiniteTrees.PossiblyInfiniteList.PossiblyInfiniteList
 theorem contrapose (A B : Prop) : A → B ↔ ¬ B → ¬ A := by grind
 
 
+theorem min_le_of_mem_set (x : Nat) (S : Set Nat) (x_in : x ∈ S) : ∃ m : Nat, m ∈ S ∧ ∀ n : Nat, n ∈ S → m ≤ n := by
+
+    let S' := (fun n => S (n + 1))
+
+    induction x generalizing S with
+    | zero =>
+        exists 0, x_in
+        intro n n_in
+        exact Nat.zero_le n
+
+    | succ x ih =>
+        by_cases c : 0 ∈ S
+
+        exists 0, c
+        intro n n_in
+        exact Nat.zero_le n
+
+        have x_in' : S' x := by exact x_in
+
+        rcases ih S' x_in' with ⟨m, hm, hmin⟩
+        exists (m+1), hm
+        intro n n_in
+        cases n with
+        | zero =>
+            contradiction
+        | succ n =>
+            exact Nat.add_le_add_right (hmin n n_in) 1
+
+-- well order principle 
+theorem wop (S : Set Nat) (S_non_empty : ∃ (n : Nat), n ∈ S) : ∃ (m : Nat), m ∈ S ∧ ∀ (n : Nat), n ∈ S → m ≤ n := by
+  rcases S_non_empty with ⟨n, h⟩
+  exact min_le_of_mem_set n S h
+
+
+/-
+  l = [x1, x2, x3, x4]
+
+  y1 = f init x1
+  y2 = f y1 x2
+  y3 = f y2 x3
+
+  foldl_save_hist l init f = [init, (f init x1), (f (f init x1) x2), (f (f (f init x1) x2) x3)]
+
+  foldl_save_hist l init f = [init, y1, y2, y3]
+
+-/
+
+def foldl_save_hist (l : List α) (init_elem : β) (f : β → α → β) : List β :=
+  let (_, history) :=
+    l.foldl
+      (fun (state, hist) t =>
+        let next := f state t
+        (next, hist.concat next))
+      (init_elem, [init_elem])
+  history
+
+-- foldl_save_hist variant for function returning options, if none is retuned by f the argument is not applied and the previous element which was some is returned
+def foldl_save_hist_opt (l : List α) (init_elem : β) (f : β → α → Option β) : List β :=
+  let (_, history) :=
+  l.foldl
+    (fun (state, hist) t =>
+      let next :=
+        match (f state t) with
+          | some s' => s'
+          | none    => state
+      (next, hist.concat next))
+    (init_elem, [init_elem])
+history
+
+def foldl_save_hist_opt_nodup [DecidableEq β] (l : List α) (init_elem : β) (f : β → α → Option β) : List β :=
+  let (_, history) :=
+    l.foldl
+      (fun (state, history) t =>
+        let next := (f state t).getD state
+        if next = state then
+          (state, history)
+        else
+          (next, history.concat next))
+      (init_elem, [init_elem])
+  history
+
+def foldl_save_hist_opt_nodup_trace [DecidableEq β] (l : List α) (init : β) (f : β → α → Option β) : List (β × Option α) :=
+  let (_, history) :=
+    l.foldl
+      (fun (state, history) o =>
+        let next := (f state o).getD state
+        if next = state then
+          (state, history)
+        else
+          (next, history.concat (next, some o)))
+      (init, [(init, none)])
+  history
+
+#eval foldl_save_hist [1, 2, 3, 0, 1] 5 (fun a b => a + b)
+
+def test_fun (a b : Nat) : Option (Nat) :=
+    if (a > b) then a - b else none
+
+#eval foldl_save_hist_opt [5, 20, 20, 1, 10, 5, 0, 1] 20 test_fun
+
+#eval foldl_save_hist_opt_nodup [5, 20, 20, 1, 10, 5, 0, 1] 20 test_fun
+
+#eval foldl_save_hist_opt_nodup_trace [5, 20, 20, 1, 10, 5, 0, 1] 20 test_fun
+
+
+@[grind =]
+theorem head_concat (l : List β) (x : β) (h : l ≠ []) :
+  (l.concat x).head? = l.head? := by
+  cases l with
+  | nil =>
+    contradiction
+  | cons hd tl =>
+    simp [List.concat]
+
+@[grind =]
+theorem foldl_save_hist_head_eq (l : List α) (init_elem : β) (f : β → α → β) :
+  (foldl_save_hist l init_elem f).head? = some init_elem := by
+    unfold foldl_save_hist
+    have h : ∀ (l : List α) (state : β) (hist : List β),
+      hist.head? = some init_elem → (l.foldl (fun (state, hist) t =>
+        let next := f state t
+        (next, hist.concat next))
+        (state, hist)).snd.head? = some init_elem := by
+          intro l
+          induction l with
+          | nil =>
+            grind
+          | cons hd tl ih =>
+            grind
+
+    exact h l init_elem [init_elem] rfl
+
+theorem foldl_save_hist_opt_head_eq (l : List α) (init_elem : β) (f : β → α → Option β) :
+  (foldl_save_hist_opt l init_elem f).head? = some init_elem := by
+    unfold foldl_save_hist_opt
+    have h : ∀ (l : List α) (state : β) (hist : List β),
+      hist.head? = some init_elem → (l.foldl (fun (state, hist) t =>
+        let next := (f state t).getD state
+        (next, hist.concat next))
+        (state, hist)).snd.head? = some init_elem := by
+          intro l
+          induction l with
+            | nil =>
+              grind
+            | cons hd tl ih =>
+              grind
+
+    exact h l init_elem [init_elem] rfl
+
+theorem foldl_save_hist_opt_nodup_head_eq [DecidableEq β] (l : List α) (init_elem : β) (f : β → α → Option β) :
+(foldl_save_hist_opt_nodup l init_elem f).head? = some init_elem := by
+  unfold foldl_save_hist_opt_nodup
+  have h : ∀ (l : List α) (state : β) (hist : List β),
+    hist.head? = some init_elem → (l.foldl (fun (state, hist) t =>
+      let next := (f state t).getD state
+      if next = state then
+        (state, hist)
+      else
+        (next, hist.concat next))
+      (state, hist)).snd.head? = some init_elem := by
+        intro l
+        induction l with
+          | nil =>
+            grind
+          | cons hd tl ih =>
+            grind
+
+  exact h l init_elem [init_elem] rfl
+
+
+@[grind =]
+theorem head?_eraseDups [DecidableEq α] (l : List α) (h : l ≠ []) :
+  (l.eraseDups).head? = l.head? := by
+    induction l with
+      | nil =>
+        contradiction
+      | cons x xs =>
+        simp only [List.head?_cons]
+        grind
+
+
+@[grind .]
+theorem foldl_save_hist_opt_nodup_trace_adjacent_ne [DecidableEq β] (l : List α) (init : β) (f : β → α → Option β) (n : Nat) (h : n + 1 < (foldl_save_hist_opt_nodup_trace l init f).length) :
+  (foldl_save_hist_opt_nodup_trace l init f)[n] ≠ (foldl_save_hist_opt_nodup_trace l init f)[n+1] := by
+    intro contra
+    let hist := foldl_save_hist_opt_nodup_trace l init f
+    have hist_eq : hist[n] = hist[n+1] := contra
+
+    have hstep :
+      ∃ (state next : β) (o : Option α),
+        hist[n] = (state, o) ∧
+        hist[n+1] = (next, o) ∧
+        next ≠ state := by
+
+      have : ∃ (state next : β) (o : Option α),
+        (foldl_save_hist_opt_nodup_trace l init f)[n]'(Nat.lt_of_succ_lt h) = (state, o) ∧
+        (foldl_save_hist_opt_nodup_trace l init f)[n+1]'(by exact Nat.lt_of_succ_le h) = (next, o) ∧
+        next ≠ state := by
+
+          induction l generalizing n with
+          | nil =>
+            exists init
+          | cons hd tl ih =>
+            sorry
+      exact this
+    -- contradiciton of state = next and state ≠ next
+    grind
+
 namespace Function
 
   theorem id_is_injective (A : Set α) : Function.injective_for_domain_set id A := by
